compiler/src/FlatToRiscvBW.v
@@ -1,0 +1,187 @@
+Require Import lib.LibTacticsMin.
+Require Import riscv.Utility.Monads. Require Import riscv.Utility.MonadNotations.
+Require Import coqutil.Macros.unique.
+Require Import compiler.FlatImp.
+Require Import Coq.Lists.List.
+Import ListNotations.
+Require Import Coq.ZArith.ZArith.
+Require Import riscv.Spec.Machine.
+Require Import riscv.Spec.Decode.
+Require Import riscv.Spec.PseudoInstructions.
+Require Import riscv.Platform.RiscvMachine.
+Require Import riscv.Spec.Execute.
+Require Import riscv.Platform.Run.
+Require Import riscv.Platform.Memory.
+Require Import riscv.Utility.PowerFunc.
+Require Import riscv.Utility.ListLib.
+Require Import coqutil.Decidable.
+Require Import Coq.Program.Tactics.
+Require Import Coq.Bool.Bool.
+Require Import riscv.Utility.InstructionCoercions.
+Require Import riscv.Spec.Primitives.
+Require Import Coq.micromega.Lia.
+Require Import riscv.Utility.div_mod_to_quot_rem.
+Require Import compiler.util.Misc.
+Require Import riscv.Utility.Utility.
+Require Import riscv.Utility.ZBitOps.
+Require Import compiler.util.Common.
+Require Import riscv.Utility.Utility.
+Require Import riscv.Utility.MkMachineWidth.
+Require Import riscv.Utility.runsToNonDet.
+Require Import compiler.Rem4.
+Require Import compiler.FlatToRiscvDef.
+Require Import compiler.GoFlatToRiscv.
+Require Import compiler.EmitsValid.
+Require Import compiler.SeparationLogic.
+Require Import bedrock2.Scalars.
+Require Import compiler.Simp.
+Require Import compiler.SimplWordExpr.
+
+Local Open Scope ilist_scope.
+Local Open Scope Z_scope.
+
+
+Module Import FlatToRiscvBW.
+  Export FlatToRiscvDef.FlatToRiscvDef.
+
+  Class parameters(width: Z)(width_cases: width = 32 \/ width = 64) := {
+    byte :> word.word 8;
+    byte_ok :> word.ok byte;
+    word :> word.word width;
+    word_ok :> word.ok word;
+
+    W :> Utility.Words := {|
+      Utility.byte := byte;
+      Utility.byte_ok := byte_ok;
+      Utility.width := width;
+      Utility.width_cases := width_cases;
+      Utility.word := word;
+      Utility.word_ok := word_ok;
+    |};
+
+    actname : Type;
+    compile_ext_call : list Register -> actname -> list Register -> list Instruction;
+    max_ext_call_code_size : actname -> Z;
+    compile_ext_call_length : forall (binds : list Register) (f : actname) (args : list Register),
+                              Zlength (compile_ext_call binds f args) <= max_ext_call_code_size f;
+    compile_ext_call_emits_valid : forall (iset : InstructionSet) (binds : list Register)
+                                     (a : actname) (args : list Register),
+                                   Forall valid_register binds ->
+                                   Forall valid_register args ->
+                                   valid_instructions iset (compile_ext_call binds a args);
+
+    locals :> map.map Register word;
+    locals_ok :> map.ok locals;
+    mem :> map.map word byte;
+    mem_ok :> map.ok mem;
+
+    M: Type -> Type;
+    MM :> Monad M;
+
+    RVM :> RiscvProgram M word;
+    PRParams :> PrimitivesParams M (RiscvMachine Register actname);
+    PR :> Primitives PRParams;
+  }.
+
+  Instance def_params{width: Z}{width_cases: width = 32 \/ width = 64}
+        (p: parameters width width_cases): FlatToRiscvDef.parameters := {
+    FlatToRiscvDef.FlatToRiscvDef.actname := actname;
+    FlatToRiscvDef.FlatToRiscvDef.compile_ext_call := compile_ext_call;
+    FlatToRiscvDef.FlatToRiscvDef.max_ext_call_code_size := max_ext_call_code_size;
+    FlatToRiscvDef.FlatToRiscvDef.compile_ext_call_length := compile_ext_call_length;
+    FlatToRiscvDef.FlatToRiscvDef.compile_ext_call_emits_valid := compile_ext_call_emits_valid;
+  }.
+
+  Class proofs{width: Z}{width_cases: width = 32 \/ width = 64}
+        (p: parameters width width_cases) := {
+    go_load: forall sz x a (addr v: word) initialL post f,
+      valid_register x ->
+      valid_register a ->
+      map.get initialL.(getRegs) a = Some addr ->
+      Memory.load sz (getMem initialL) addr = Some v ->
+      mcomp_sat (f tt)
+                (withRegs (map.put initialL.(getRegs) x v) initialL) post ->
+      mcomp_sat (Bind (execute (compile_load sz x a 0)) f) initialL post;
+
+   go_store: forall sz x a (addr v: word) initialL m' post f,
+      valid_register x ->
+      valid_register a ->
+      map.get initialL.(getRegs) x = Some v ->
+      map.get initialL.(getRegs) a = Some addr ->
+      Memory.store sz (getMem initialL) addr v = Some m' ->
+      mcomp_sat (f tt) (withMem m' initialL) post ->
+      mcomp_sat (Bind (execute (compile_store sz a x 0)) f) initialL post;
+  }.
+
+End FlatToRiscvBW.
+
+
+Section Proofs32.
+  Context (p: FlatToRiscvBW.parameters 32 (or_introl eq_refl)).
+
+  Arguments LittleEndian.combine: simpl never.
+
+  Instance Proofs32: proofs p.
+  Proof.
+    constructor.
+    - intros. unfold compile_load.
+      destruct sz;
+        unfold execute, ExecuteI.execute, ExecuteI64.execute, translate, DefaultRiscvState,
+        Memory.load, Memory.load_Z in *;
+        simp; simulate; simpl; simpl_word_exprs word_ok;
+          try eassumption.
+    - intros. unfold compile_store.
+      destruct sz;
+        unfold execute, ExecuteI.execute, ExecuteI64.execute, translate, DefaultRiscvState,
+        Memory.store, Memory.store_Z in *;
+        simp; simulate; simpl; simpl_word_exprs word_ok; eassumption.
+  Qed.
+
+End Proofs32.
+
+
+Section Proofs64.
+  Context (p: FlatToRiscvBW.parameters 64 (or_intror eq_refl)).
+
+  Arguments LittleEndian.combine: simpl never.
+
+  Instance Proofs64: proofs p.
+  Proof.
+    constructor.
+    - intros. unfold compile_load.
+      destruct sz;
+        unfold execute, ExecuteI.execute, ExecuteI64.execute, translate, DefaultRiscvState,
+        Memory.load, Memory.load_Z in *;
+        simp; simulate; simpl; simpl_word_exprs word_ok;
+          eassumption.
+    - intros. unfold compile_store.
+      destruct sz;
+        unfold execute, ExecuteI.execute, ExecuteI64.execute, translate, DefaultRiscvState,
+        Memory.store, Memory.store_Z in *;
+        simp; simulate; simpl; simpl_word_exprs word_ok; eassumption.
+  Qed.
+
+End Proofs64.
+
+Lemma ProofsBWHelper:
+  forall (is32Bit: bool),
+    let width: Z := if is32Bit then 32 else 64 in
+    let width_cases: width = 32 \/ width = 64 :=
+        if is32Bit as b return ((if b then 32 else 64) = 32 \/ (if b then 32 else 64) = 64)
+        then or_introl eq_refl
+        else or_intror eq_refl in
+    forall (p: FlatToRiscvBW.parameters width width_cases), proofs p.
+Proof.
+  intro is32Bit. case is32Bit; simpl.
+  - exact Proofs32.
+  - exact Proofs64.
+Qed.
+
+Instance ProofsBW:
+  forall (width: Z) (width_cases: width = 32 \/ width = 64)
+         (p: FlatToRiscvBW.parameters width width_cases), proofs p.
+Proof.
+  intros width width_cases. destruct width_cases as [C | C].
+  - pose proof (ProofsBWHelper true) as P. simpl in P. rewrite C. exact P.
+  - pose proof (ProofsBWHelper false) as P. simpl in P. rewrite C. exact P.
+Qed.
