compiler/src/examples/InlineAssemblyMacro.v
@@ -113,6 +113,6 @@ Instance compilation_params: FlatToRiscvDef.parameters := {|
   FlatToRiscvDef.max_ext_call_code_size _ := 100;
 |}. all: case TODO. Defined.
 
-Definition compiled: list Instruction := Eval cbv in compile_stmt RV32IM test.
+Definition compiled: list Instruction := Eval cbv in compile_stmt test.
 
 Print compiled.
